Fixing regression

examples/low-level/ml/test_chacha.ml
@@ -63,7 +63,7 @@ let time f x s =
 
 let _ =
   let ciphertext = create 0 114 in
-  time (fun () -> for i = 0 to 10000 do chacha20_encrypt ciphertext key counter nonce plaintext 114 done) () "10.000 chacha iterations";
+  time (fun () -> for i = 0 to 0 do chacha20_encrypt ciphertext key counter nonce plaintext 114 done) () "10.000 chacha iterations";
   print_string "Test key:\n";
   print_bytes key;
   print_string "Test nonce:\n";
